Cleanup.

csdl.v
@@ -1,22 +1,16 @@
 Require Import CSDL.Basics CSDL.Binary String.
+Require Import EquivDec Bool SetoidTactics.
  (* Program Equations Bvector List Arith Euclid Omega. *)
 
 Definition ty := nat.
 Definition const := bits.
 
-Fixpoint type_of_op (l : list ty) (t : ty) :=
+Fixpoint operator (l : list ty) (t : ty) :=
   match l with
     | nil => const t
-    | t' :: l' => const t' -> type_of_op l' t
+    | t' :: l' => const t' -> operator l' t
   end.
-
-Inductive operator (l : list ty) (t : ty) : Set :=
-| OP (op : type_of_op l t).
   
-(* Class Operator (A : Type) (a : A) := *)
-(*   { args : list ty ; *)
-(*     res *)
-
 Inductive endianness := BigEndian | LittleEndian.
 
 Record space := mkSpace {
@@ -27,34 +21,6 @@ Record space := mkSpace {
 }.
 
 Existing Instance space_cell_size_pos.
-  
-(* Variable space : Π (number : option nat) (addressing : ty) (size : ty), Set. *)
-
-Inductive loc (n : ty) : Set := LOC (b : bits n).
-
-Variable cells : nat -> Set. 
-
-(* Record cells (t : ty) := CELLS  *)
-(*   { cell_num : option nat; *)
-(*     cell_adressing : ty; *)
-(*     (* cell_start: loc a; *) *)
-(*     cell_space : space cell_num cell_adressing t }. *)
-
-Definition lift_const {t : ty} (c : nat) `{r : Representable t c} : const t :=
-  representation t c.
-
-(* Instance: Have (w > n) -> Have (w > 0). *)
-(* Proof. unfold Have ; intros ; omega. Qed. *)
-
-(* Goal Have (2 > 0). *)
-(*   progress eapply @Have_instance_0. *)
-(*   progress eapply @Have_instance_0. *)
-(*   progress eapply @Have_instance_0. *)
-(*   progress eapply @Have_instance_0. *)
-(*   progress eapply @Have_instance_0. *)
-
-
-
 
 Inductive exp : ty -> Set :=
 | CONST {n : ty} (c : const n) : exp n
@@ -70,13 +36,6 @@ with location : ty -> Set :=
   `{wgtn : Have (w > s.(space_cell_size))}
   `{wmultn : Have (modulo_nat w s.(space_cell_size) = 0)} : location w.
 
-(* with location : ty -> Set := *)
-(* | AGG {n w} (b : endianness) (c : cell n) `{wgtn : Have (w > n)} `{Have (n > 0)} *)
-(*   `{wmultn : Have (modulo_nat w n = 0)} : location w *)
-
-(* with cell : ty -> Set := *)
-(* | CELL (s : space) (e : exp s.(space_address)) : cell s.(space_cell_size). *)
-
 Inductive effect : Set :=
 | STORE {n} (dst : location n) (src : exp n)
 | KILL {n} (l : location n).
@@ -85,8 +44,6 @@ Inductive guarded : Set :=
 | GUARD {n} (e : exp n) (ef : effect).
 
 Definition rtl := list guarded.
-
-Definition cell_name := string.
 
 Definition space_descr (sp : space) :=
   const sp.(space_address) -> forall agg : nat, option (bits (agg * sp.(space_cell_size))).
@@ -105,9 +62,6 @@ Definition bind {A B} (x : interpM A) (y : A -> interpM B) : interpM B :=
       | None => (None, s')
       | Some c => y c s'
     end.
-
-Axiom cheat : Π {α}, α.
-
 
 Notation " ( x &? ) " := (exist _ x _).
 
@@ -138,20 +92,19 @@ with eval_exp {n} (e : exp n) : interpM (const n) :=
   match e with
     | CONST n c => ret c
     | FETCH n l => eval_fetch l
-    | APP l n o es => 
-      let 'OP f := o in
-        (fix aux l (es : args l) : type_of_op l n -> interpM (const n) :=
-          match es in args l return type_of_op l n -> interpM (const n) with
-            | ARGnil => fun op => ret op
-            | ARGcons ty tys e es => fun op => 
-              bind (eval_exp e) (fun e' =>
-                aux tys es (op e'))
-          end) l es f
+    | APP l n f es => 
+      (fix aux l (es : args l) : operator l n -> interpM (const n) :=
+        match es in args l return operator l n -> interpM (const n) with
+          | ARGnil => fun op => ret op
+          | ARGcons ty tys e es => fun op => 
+            bind (eval_exp e) (fun e' =>
+              aux tys es (op e'))
+        end) l es f
   end.
 
-Definition eval_app {n : ty} {l : list ty} (es : args l) : type_of_op l n -> interpM (const n) :=
-  (fix aux l (es : args l) : type_of_op l n -> interpM (const n) :=
-  match es in args l return type_of_op l n -> interpM (const n) with
+Definition eval_app {n : ty} {l : list ty} (es : args l) : operator l n -> interpM (const n) :=
+  (fix aux l (es : args l) : operator l n -> interpM (const n) :=
+  match es in args l return operator l n -> interpM (const n) with
     | ARGnil => fun op => ret op
     | ARGcons ty tys e es => fun op => 
       bind (eval_exp e) (fun e' => aux tys es (op e'))
@@ -169,73 +122,20 @@ Lemma eval_fetch_agg {w} (endian : endianness) (sp : space) e wgtn wmultn :
     (mem_cell_fetches_agg mem endian sp c wgtn _ wmultn, mem)).
 Proof. trivial. Qed.
 
-Lemma eval_exp_app {l : list ty} {n : ty} (o : type_of_op l n) (es : args l) :
-  eval_exp (APP (OP l n o) es) = eval_app es o.
+Lemma eval_exp_app {l : list ty} {n : ty} (o : operator l n) (es : args l) :
+  eval_exp (APP o es) = eval_app es o.
 Proof. intros. simpl. unfold eval_app. trivial. Qed.
 
-Lemma eval_app_nil {n : ty} (o : type_of_op nil n) : eval_app ARGnil o = ret o.
+Lemma eval_app_nil {n : ty} (o : operator nil n) : eval_app ARGnil o = ret o.
 Proof. intros. trivial. Qed.
 
-Lemma eval_app_cons {t : ty} {l : list ty} (e : exp t) (es : args l) {n : ty} (o : type_of_op (t :: l) n) : 
+Lemma eval_app_cons {t : ty} {l : list ty} (e : exp t) (es : args l) {n : ty} (o : operator (t :: l) n) : 
   eval_app (ARGcons e es) o = bind (eval_exp e) (fun e' => eval_app es (o e')).
 Proof. intros. trivial. Qed.
 
-Equations(nocomp) binary_eq {n} (x y : const n) : bool :=
-binary_eq ?(0) Vnil Vnil := true ;
-binary_eq ?(S n) (Vcons a n x) (Vcons b n y) := bool_eq a b && binary_eq x y.
-
-(* Equations(nocomp) binary_eq {n} (x y : const n) : { x = y } + { x <> y } := *)
-(* binary_eq ?(0) Vnil Vnil := left eq_refl ; *)
-(* binary_eq ?(S n) (Vcons true n x) (Vcons true n y) := if binary_eq x y then in_left else in_right ; *)
-(* binary_eq ?(S n) (Vcons false n x) (Vcons false n y) := if binary_eq x y then in_left else in_right ; *)
-(* binary_eq ?(S n) (Vcons a n _) (Vcons b n _) := in_right. *)
-
-Require Import EquivDec Bool.
 Instance space_eq : EqDec space eq.
 Admitted.
 
-Lemma bool_eq_refl b : bool_eq b b = true.
-Proof. destruct b ; reflexivity. Qed.
-
-Lemma binary_eq_refl n (b : const n) : binary_eq b b = true.
-Proof. intros. remember b as b'. rewrite Heqb' at 1. funind (binary_eq b b') foo. 
-  rewrite bool_eq_refl. rewrite IHbinary_eq_ind. reflexivity.
-  simp binary_eq in foo. rewrite bool_eq_refl in foo. assumption.
-Qed.
-
-Instance const_eq : EqDec (const n) eq.
-Proof. 
-intros n. red. intros. case_eq (binary_eq x y) ; [ left | right ].
-
-  funind (binary_eq x y) foo. reflexivity.
-  red. rewrite andb_true_iff in x. destruct x.
-  specialize (IHbinary_eq_ind H1).
-  apply bool_eq_ok in H. subst.
-  simp binary_eq in foo. rewrite bool_eq_refl in foo. 
-  specialize (IHbinary_eq_ind foo). congruence.
-
-  funind (binary_eq x y) foo. red ; intros.
-  red in H. noconf H. simp binary_eq in foo.
-  rewrite bool_eq_refl, binary_eq_refl in foo.
-  simpl in foo. discriminate.
-Qed.
-  
-Definition coerce_bits {n m} (c : bits n) (H : n = m) : bits m.
-Proof. intros ; subst. exact c. Defined.
-
-Equations(nocomp) vector_firstn {A} {l : nat} (s : nat) (c : vector A l) (Hsl : s < l) : vector A s :=
-vector_firstn A ?(O) s Vnil Hsl :=! Hsl ;
-vector_firstn A ?(S n) O (Vcons a n v) Hsl := Vnil ;
-vector_firstn A ?(S n) (S m) (Vcons a n v) Hsl := Vcons a (vector_firstn m v _).
-
-  Next Obligation. omega. Defined.
-
-  Next Obligation. revert s Hsl ; induction c ; intros ;
-    simp vector_firstn ; auto with * ; destruct s ; simp vector_firstn.
-  Defined.
-
-Require Import Morphisms SetoidTactics.
-  
 Definition mem_cell_store_agg {w} (m : mem) (e : endianness) (sp : space) (addr : const sp.(space_address)) 
   (c : option (const w))
   `{wgtn : Have (w > sp.(space_cell_size))} `{Have (sp.(space_cell_size) > 0)}
@@ -290,9 +190,6 @@ Equations(nocomp) apply_effect (e : effect) : interpM () :=
 apply_effect (STORE n dst src) :=
   bind (eval_exp src) (fun e' => eval_store dst (Some e')) ;
 apply_effect (KILL n l) := eval_store l None.
-
-Definition one_binary_le {n : nat} : const n := 
-  fst (bits_succ _ (constant_vector n false)).
     
 Definition one_guarded (g : guarded) : interpM () :=
   let 'GUARD n e ef := g in
@@ -307,10 +204,3 @@ Definition seq (x y : interpM ()) :=
 
 Definition eval_rtl (r : rtl) : interpM () :=
   fold_left (fun acc g => seq acc (one_guarded g)) r (ret ()).
-
-
-
-
-
-
-
